code/ecdsap256/Hacl.Impl.ECDSA.P256.Verification.Agile.fst
@@ -139,7 +139,7 @@ let ecdsa_verification_step23 #c alg mLen m result =
   reduction_prime_2prime_order result result;
 
   lemma_core_0 c result h1;
-  changeEndianLemma (uints_from_bytes_be #U64 #_ #4 (as_seq h1 cutHash));
+  changeEndianLemma #c (uints_from_bytes_be #U64 #_ #4 (as_seq h1 cutHash));
   uints_from_bytes_be_nat_lemma #U64 #_ #4 (as_seq h1 cutHash);
 
   pop_frame()
@@ -202,24 +202,24 @@ let ecdsa_verification_step4 #c bufferU1 bufferU2 r s hash =
     calc(==) {
     as_seq h2 bufferU1;
     == {}
-    uints_to_bytes_be (changeEndian (as_seq h1 u1));
+    uints_to_bytes_be (Hacl.Spec.P256.Definition.changeEndian #c (as_seq h1 u1));
     == {lemma_nat_from_to_intseq_le_preserves_value 4 (as_seq h1 u1)}
-    uints_to_bytes_be (changeEndian (nat_to_intseq_le 4 (nat_from_intseq_le (as_seq h1 u1))));
+    uints_to_bytes_be (Hacl.Spec.P256.Definition.changeEndian #c (nat_to_intseq_le 4 (nat_from_intseq_le (as_seq h1 u1))));
     == {lemma_core_0 c u1 h1}
-    uints_to_bytes_be (changeEndian (nat_to_intseq_le 4 (as_nat c h1 u1)));
-    == { changeEndian_le_be (as_nat c h1 u1) }
+    uints_to_bytes_be (Hacl.Spec.P256.Definition.changeEndian #c (nat_to_intseq_le 4 (as_nat c h1 u1)));
+    == {changeEndian_le_be #c (as_nat c h1 u1) }
     nat_to_bytes_be 32 (as_nat c h1 u1);
     };
 
     calc(==) {
       as_seq h2 bufferU2;
       == {}
-      uints_to_bytes_be (changeEndian (as_seq h1 u2));
+      uints_to_bytes_be (Hacl.Spec.P256.Definition.changeEndian #c (as_seq h1 u2));
       == {lemma_nat_from_to_intseq_le_preserves_value 4 (as_seq h1 u2)}
-      uints_to_bytes_be (changeEndian (nat_to_intseq_le 4 (nat_from_intseq_le (as_seq h1 u2))));
+      uints_to_bytes_be (Hacl.Spec.P256.Definition.changeEndian #c (nat_to_intseq_le 4 (nat_from_intseq_le (as_seq h1 u2))));
       == {lemma_core_0 c u2 h1}
-      uints_to_bytes_be (changeEndian (nat_to_intseq_le 4 (as_nat c h1 u2)));
-      == { changeEndian_le_be (as_nat c h1 u2) }
+      uints_to_bytes_be (Hacl.Spec.P256.Definition.changeEndian #c (nat_to_intseq_le 4 (as_nat c h1 u2)));
+      == {changeEndian_le_be #c (as_nat c h1 u2) }
       nat_to_bytes_be 32 (as_nat c h1 u2);
     };
 
@@ -586,16 +586,16 @@ let ecdsa_verification c alg pubKey r s mLen m =
     let result = ecdsa_verification_ #c alg publicKeyAsFelem rAsFelem sAsFelem mLen m in 
     pop_frame();
 
-    changeEndianLemma (uints_from_bytes_be (as_seq h1 (gsub pubKey (size 0) (size 32))));
+    changeEndianLemma #c (uints_from_bytes_be (as_seq h1 (gsub pubKey (size 0) (size 32))));
     uints_from_bytes_be_nat_lemma #U64 #_ #4 (as_seq h1 (gsub pubKey (size 0) (size 32)));
     
-    changeEndianLemma (uints_from_bytes_be (as_seq h1 (gsub pubKey (size 32) (size 32))));
+    changeEndianLemma #c (uints_from_bytes_be (as_seq h1 (gsub pubKey (size 32) (size 32))));
     uints_from_bytes_be_nat_lemma #U64 #_ #4 (as_seq h1 (gsub pubKey (size 32) (size 32)));
     
-    changeEndianLemma (uints_from_bytes_be (as_seq h1 r));
+    changeEndianLemma #c (uints_from_bytes_be (as_seq h1 r));
     uints_from_bytes_be_nat_lemma #U64 #_ #4 (as_seq h1 r);
     
-    changeEndianLemma (uints_from_bytes_be (as_seq h1 s));
+    changeEndianLemma #c (uints_from_bytes_be (as_seq h1 s));
     uints_from_bytes_be_nat_lemma #U64 #_ #4 (as_seq h1 s);
 
   result
