code/ecdsap256/Hacl.Impl.P256.Signature.Common.fst
@@ -370,10 +370,10 @@ let verifyQ #c pubKey =
       lemma_core_0 c publicKeyY h1;
       uints_from_bytes_le_nat_lemma #U64 #SEC #4 (as_seq h1 pubKeyY); 
 
-      changeEndianLemma (uints_from_bytes_be (as_seq h1 (gsub pubKey (size 0) (size 32))));
+      changeEndianLemma #c (uints_from_bytes_be (as_seq h1 (gsub pubKey (size 0) (size 32))));
       uints_from_bytes_be_nat_lemma #U64 #_ #4 (as_seq h1 (gsub pubKey (size 0) (size 32)));
       
-      changeEndianLemma (uints_from_bytes_be (as_seq h1 (gsub pubKey (size 32) (size 32))));
+      changeEndianLemma #c (uints_from_bytes_be (as_seq h1 (gsub pubKey (size 32) (size 32))));
       uints_from_bytes_be_nat_lemma #U64 #_ #4 (as_seq h1 (gsub pubKey (size 32) (size 32)));
 
   bufferToJac #c publicKeyB publicKeyJ;
